Change argument order in uniformize_fun and replace_tm to that of uniformize

Escallon/Chomsky_Normal_Form_Fun/Chomsky_Normal_Form_Fun.thy
@@ -22,34 +22,34 @@ proof -
   finally show ?thesis .
 qed
 
-fun replace_tm :: "['t, 'n, ('n,'t) syms] \<Rightarrow> ('n,'t) syms" where
-  "replace_tm t A [] = []" |
-  "replace_tm t A (s # sms) = (if s = Tm t then Nt A # sms else s # replace_tm t A sms)"
+fun replace_tm :: "['n, 't, ('n,'t) syms] \<Rightarrow> ('n,'t) syms" where
+  "replace_tm A t [] = []" |
+  "replace_tm A t (s # sms) = (if s = Tm t then Nt A # sms else s # replace_tm A t sms)"
 
 lemma replace_tm_length_unchanged[simp]: 
-  "length (replace_tm t A sms) = length sms"
+  "length (replace_tm A t sms) = length sms"
   by (induction sms) auto
   
 
 lemma replace_tm_id_iff_tm_notin_syms:
-  shows "Tm t \<notin> set sms \<longleftrightarrow> replace_tm t A sms = sms"
+  shows "Tm t \<notin> set sms \<longleftrightarrow> replace_tm A t sms = sms"
   by (induction sms) auto
 
 (*Proofs break with iff lemma. Fix?*)
 lemma tm_notin_syms_impl_replace_tm_id:
   assumes "Tm t \<notin> set sms" 
-  shows "replace_tm t A sms = sms"
+  shows "replace_tm A t sms = sms"
   using assms replace_tm_id_iff_tm_notin_syms by fast
 lemma replace_tm_id_impl_tm_notin_syms:
-  assumes "replace_tm t A sms = sms"
+  assumes "replace_tm A t sms = sms"
   shows "Tm t \<notin> set sms"
   using assms replace_tm_id_iff_tm_notin_syms by fast
 
 (*Strengthen with "Tm t \<notin> set p?*)
 lemma replace_tm_replaces_single:
-  assumes "replace_tm t A sms \<noteq> sms"
+  assumes "replace_tm A t sms \<noteq> sms"
   obtains p s where "sms = p@[Tm t]@s"
-                    "replace_tm t A sms = p@[Nt A]@s"
+                    "replace_tm A t sms = p@[Nt A]@s"
 using assms proof (induction sms arbitrary: thesis)
   case (Cons s sms)
   from Cons(3) have t_in_ssms: "Tm t \<in> set (s#sms)" using replace_tm_id_iff_tm_notin_syms by fast
@@ -58,15 +58,15 @@ using assms proof (induction sms arbitrary: thesis)
   proof cases
     case eq
     then obtain p q where "s#sms = p@[Tm t]@q" "p = []" by auto
-    moreover from eq have "replace_tm t A (s#sms) = Nt A#sms" by simp
+    moreover from eq have "replace_tm A t (s#sms) = Nt A#sms" by simp
     ultimately show thesis using Cons(2) by fastforce
   next
     case neq
     with t_in_ssms have "Tm t \<in> set sms" 
       by simp
     with Cons(1) replace_tm_id_iff_tm_notin_syms 
-    obtain p q where pq_defs: "sms = p@[Tm t]@q" "replace_tm t A sms = p@[Nt A]@q" by metis
-    with neq have "replace_tm t A (s#sms) = (s#p)@[Nt A]@q" by auto
+    obtain p q where pq_defs: "sms = p@[Tm t]@q" "replace_tm A t sms = p@[Nt A]@q" by metis
+    with neq have "replace_tm A t (s#sms) = (s#p)@[Nt A]@q" by auto
     then show ?thesis using Cons(2) pq_defs by (meson Cons_eq_appendI)
   qed
 qed simp
@@ -76,38 +76,38 @@ qed simp
 
 (*The current implementation corresponds to uniformize as defined in 
   Context_Free_Grammar.Chomsky_Normal_Form. This can be simplified with maps.*)
-fun uniformize_fun :: "['t, 'n, ('n,'t) prods, ('n,'t) prods] \<Rightarrow> ('n,'t) prods" where
+fun uniformize_fun :: "['n, 't, ('n,'t) prods, ('n,'t) prods] \<Rightarrow> ('n,'t) prods" where
   "uniformize_fun _ _ ps0 [] = ps0" |
-  "uniformize_fun t A ps0 ((l,r) # ps) = 
-    (let r' = replace_tm t A r in 
-      if r = r' \<or> length r < 2 then uniformize_fun t A ps0 ps
+  "uniformize_fun A t ps0 ((l,r) # ps) = 
+    (let r' = replace_tm A t r in 
+      if r = r' \<or> length r < 2 then uniformize_fun A t ps0 ps
       else (removeAll (l,r) ps0) @ [(A, [Tm t]), (l,r')])"
 
 lemma uniformize_fun_id:
   assumes "\<forall>(l,r)\<in>set ps. Tm t \<notin> set r \<or> length r < 2"
-  shows "uniformize_fun t A ps0 ps = ps0"
+  shows "uniformize_fun A t ps0 ps = ps0"
   using assms tm_notin_syms_impl_replace_tm_id by (induction ps) fastforce+
 
 lemma uniformize_fun_uniform_prepend:
    "\<forall>(l,r)\<in>set xs. Tm t \<notin> set r \<or> length r < 2 \<Longrightarrow>
-    uniformize_fun t A ps0 (xs@ps) = uniformize_fun t A ps0 ps"
+    uniformize_fun A t ps0 (xs@ps) = uniformize_fun A t ps0 ps"
 proof (induction xs)
   case (Cons x xs)
   then obtain l r where lr_def: "x = (l,r)" by auto
-  hence "uniformize_fun t A ps0 ((x#xs)@ps) = uniformize_fun t A ps0 ((l,r)#xs@ps)" by simp
-  also have "... = uniformize_fun t A ps0 (xs@ps)"
+  hence "uniformize_fun A t ps0 ((x#xs)@ps) = uniformize_fun A t ps0 ((l,r)#xs@ps)" by simp
+  also have "... = uniformize_fun A t ps0 (xs@ps)"
   proof -
     from Cons(2) lr_def have "Tm t \<notin> set r \<or> length r < 2" by simp
-    hence "replace_tm t A r = r \<or> length r < 2" using tm_notin_syms_impl_replace_tm_id by fast
+    hence "replace_tm A t r = r \<or> length r < 2" using tm_notin_syms_impl_replace_tm_id by fast
     thus ?thesis by auto
   qed
-  also have "... = uniformize_fun t A ps0 ps" using Cons by simp
+  also have "... = uniformize_fun A t ps0 ps" using Cons by simp
   finally show ?case .
 qed simp
 
 lemma uniformize_fun_ps0_uniform_app:
   assumes "\<forall>(l,r)\<in>set xs. Tm t \<notin> set r \<or> length r < 2"
-  shows "uniformize_fun t A (xs@ys) ps = xs @ uniformize_fun t A ys ps"
+  shows "uniformize_fun A t (xs@ys) ps = xs @ uniformize_fun A t ys ps"
 proof (induction ps)
   case (Cons p ps)
   then obtain l r where lr_def: "p = (l,r)" 
@@ -118,33 +118,33 @@ proof (induction ps)
   proof cases
     case not_unif
     with assms(1) lr_def have p_notin_xs: "p \<notin> set xs" by auto
-    from not_unif lr_def have "uniformize_fun t A (xs@ys) (p#ps) 
-                      = removeAll p (xs@ys) @ [(A, [Tm t]), (l,replace_tm t A r)]" 
+    from not_unif lr_def have "uniformize_fun A t (xs@ys) (p#ps) 
+                      = removeAll p (xs@ys) @ [(A, [Tm t]), (l,replace_tm A t r)]" 
       by (smt (verit) replace_tm_id_iff_tm_notin_syms uniformize_fun.simps(2)
           verit_comp_simplify1(3))
-    also have "... = xs @ removeAll p ys @ [(A, [Tm t]), (l,replace_tm t A r)]"
+    also have "... = xs @ removeAll p ys @ [(A, [Tm t]), (l,replace_tm A t r)]"
       using p_notin_xs by simp
-    also have "... = xs @ uniformize_fun t A ys (p#ps)" using not_unif 
+    also have "... = xs @ uniformize_fun A t ys (p#ps)" using not_unif 
       by (smt (verit) lr_def replace_tm_id_impl_tm_notin_syms
           uniformize_fun.simps(2) verit_comp_simplify1(3))
     finally show ?thesis .
   next
     case unif
-    hence unif_ite: "replace_tm t A r = r \<or> length r < 2" using tm_notin_syms_impl_replace_tm_id 
+    hence unif_ite: "replace_tm A t r = r \<or> length r < 2" using tm_notin_syms_impl_replace_tm_id 
       by fast
-    with lr_def have "uniformize_fun t A (xs@ys) (p#ps) = uniformize_fun t A (xs@ys) ps" 
+    with lr_def have "uniformize_fun A t (xs@ys) (p#ps) = uniformize_fun A t (xs@ys) ps" 
       by fastforce
-    also have "... = xs @ uniformize_fun t A ys ps" using Cons .
-    also have "... = xs @ uniformize_fun t A ys (p#ps)" using unif_ite lr_def by fastforce
+    also have "... = xs @ uniformize_fun A t ys ps" using Cons .
+    also have "... = xs @ uniformize_fun A t ys (p#ps)" using unif_ite lr_def by fastforce
     finally show ?thesis .
   qed
 qed simp
   
 
 lemma uniformize_fun_neq_ps0_impl_uniformized:
-  assumes "uniformize_fun t A ps0 ps \<noteq> ps0"
+  assumes "uniformize_fun A t ps0 ps \<noteq> ps0"
   obtains l r q s where "(l,r) \<in> set ps"
-                    "r \<noteq> replace_tm t A r"
+                    "r \<noteq> replace_tm A t r"
                     "length r \<ge> 2"
                     "ps = q@[(l,r)]@s"
                     "\<forall>(l,r)\<in>set q. length r < 2 \<or> Tm t \<notin> set r"
@@ -156,11 +156,11 @@ using assms proof (induction ps arbitrary: thesis)
   then show ?case 
   proof cases
     case not_fst
-    hence "uniformize_fun t A ps0 (p#ps) = uniformize_fun t A ps0 ps"
+    hence "uniformize_fun A t ps0 (p#ps) = uniformize_fun A t ps0 ps"
       using lr0_def tm_notin_syms_impl_replace_tm_id by fastforce
     then obtain l r q s where lrqs_defs: 
                               "(l,r) \<in> set ps"
-                              "r \<noteq> replace_tm t A r"
+                              "r \<noteq> replace_tm A t r"
                               "length r \<ge> 2"
                               "ps = q@[(l,r)]@s"
                               "\<forall>(l,r)\<in>set q. length r < 2 \<or> Tm t \<notin> set r"
@@ -172,7 +172,7 @@ using assms proof (induction ps arbitrary: thesis)
     ultimately show ?thesis using Cons(2) by blast
   next
     case fst
-    hence "r0 \<noteq> replace_tm t A r0" find_theorems name:replace_tm
+    hence "r0 \<noteq> replace_tm A t r0" find_theorems name:replace_tm
       using replace_tm_id_impl_tm_notin_syms by metis
     with fst lr0_def show ?thesis using Cons(2)[of _ _ "[]"] by simp
   qed
@@ -180,21 +180,21 @@ qed simp
 
 lemma uniformize_fun_uniformizes_fst:
   assumes "(l,r) \<in> set ps"
-          "r \<noteq> replace_tm t A r"
+          "r \<noteq> replace_tm A t r"
           "ps = q@[(l,r)]@s"
           "\<forall>(l,r)\<in>set q. Tm t \<notin> set r \<or> length r < 2"
           "length r \<ge> 2"
           "A = fresh P"
           "nts ps \<subseteq> P"
         shows
-    "uniformize_fun t A ps ps = ((removeAll (l,r) ps) @ [(A, [Tm t]), (l, replace_tm t A r)])" 
+    "uniformize_fun A t ps ps = ((removeAll (l,r) ps) @ [(A, [Tm t]), (l, replace_tm A t r)])" 
 proof -
   from assms(3,4) uniformize_fun_ps0_uniform_app 
       uniformize_fun_uniform_prepend have
-    "uniformize_fun t A ps ps = q @ uniformize_fun t A ([(l,r)]@s) ([(l,r)]@s)" by fastforce
-  also have "... = q @ (removeAll (l,r) ([(l,r)]@s)) @ [(A, [Tm t]), (l, replace_tm t A r)]"
+    "uniformize_fun A t ps ps = q @ uniformize_fun A t ([(l,r)]@s) ([(l,r)]@s)" by fastforce
+  also have "... = q @ (removeAll (l,r) ([(l,r)]@s)) @ [(A, [Tm t]), (l, replace_tm A t r)]"
     using assms(2,5) by fastforce
-  also have "... = removeAll (l,r) ps @ [(A, [Tm t]), (l, replace_tm t A r)]"
+  also have "... = removeAll (l,r) ps @ [(A, [Tm t]), (l, replace_tm A t r)]"
   proof -
     have "(l,r) \<notin> set q" 
       using assms(2,4,5) tm_notin_syms_impl_replace_tm_id by fastforce 
@@ -204,35 +204,36 @@ proof -
 qed
 
 lemma uniformize_fun_is_uniformized:
-  assumes "uniformize_fun t A ps ps \<noteq> ps"
+  assumes "uniformize_fun A t ps ps \<noteq> ps"
           "A = fresh (nts ps \<union> {S})"
-  shows "uniformize A t S ps (uniformize_fun t A ps ps)"
+  shows "uniformize A t S ps (uniformize_fun A t ps ps)"
 proof -
   from assms obtain l r q s  where lr_in_ps: "(l,r) \<in> set ps"
-                          and replace_neq: "r \<noteq> replace_tm t A r"
+                          and replace_neq: "r \<noteq> replace_tm A t r"
                           and len_lb: "length r \<ge> 2"
                           and ps_qs: "ps = q@[(l,r)]@s"
                           and q_uniform: "\<forall>(l,r)\<in>set q. length r < 2 \<or> Tm t \<notin> set r"
     using uniformize_fun_neq_ps0_impl_uniformized 
     by (smt (verit, del_insts) case_prodI2 case_prod_conv)
   moreover obtain p s' where "r = p@[Tm t]@s'"
-                        and replace_eq_p_Nt_s: "replace_tm t A r = p@[Nt A]@s'"
+                        and replace_eq_p_Nt_s: "replace_tm A t r = p@[Nt A]@s'"
                         and "p \<noteq> [] \<or> s' \<noteq> []"
   proof -
     from replace_tm_replaces_single replace_neq obtain p s' where
       "r = p@[Tm t]@s'"
-      "replace_tm t A r = p@[Nt A]@s'"
+      "replace_tm A t r = p@[Nt A]@s'"
       by metis
     with len_lb show thesis using that by fastforce
   qed
-  moreover have "uniformize_fun t A ps ps = removeAll (l,r) ps @ [(A, [Tm t]), (l, p @ [Nt A] @ s')]" 
+  moreover have "uniformize_fun A t ps ps = removeAll (l,r) ps @ [(A, [Tm t]), (l, p @ [Nt A] @ s')]" 
     using uniformize_fun_uniformizes_fst[OF lr_in_ps replace_neq ps_qs _ len_lb assms(2)] 
     replace_eq_p_Nt_s q_uniform by auto
   ultimately show ?thesis
     unfolding uniformize_def using assms by blast
 qed
 
-definition "uniformize_rt = undefined" (*TODO*)
+fun uniformize_rt :: "['n, 't, ('n,'t) prods, ('n,'t) prods] \<Rightarrow> ('n,'t) prods" where
+  "uniformize_rt _ = undefined"(*TODO*)
 
 lemma "(\<lambda>x y. \<exists>A t. uniformize A t S x y)^** ps (uniformize_rt A t ps ps)" (*TODO*)
   sorry
